Need to understand the MoreDep chapter to use dependent types.

play-with-dependent-types/proof.v
@@ -1,18 +1,9 @@
-Import EqNotations.
-Inductive dep (n: nat) :=
-  mkDep : dep n.
+Definition useGt0 (n: nat) (witness: n > 0) : nat :=
+  10.
 
 
-Theorem equalTypes (n n': nat): n = n' -> dep n = dep n'.
-Proof.
-  intros.
-  destruct H.
-  reflexivity.
-Qed.
-
-
-Theorem equalInhabitants (n n' : nat): forall (H: n = n'),
-    (rew H in (mkDep n)) = mkDep n'.
-  intros.
-  subst. reflexivity.
-Qed.
+Definition createGt0(n: nat) : nat :=
+  match n with
+  | O => 42
+  | S(n') => useGt0 n  (#???)
+  end.
