play-with-dependent-types/cpdt-moredep.v
@@ -1,0 +1,31 @@
+(* Solving MoreDep: http://adam.chlipala.net/cpdt/html/MoreDep.html *)
+(* Required to solve dependent type code *)
+Require Import Gt.
+
+Definition useGt0 (n: nat) (witness: n > 0) : nat :=
+  10.
+
+Definition createGt0 (n : nat) : nat :=
+  match n as x return (n = x -> nat) with
+  | O => fun _ => 42
+  | S n' => fun E => useGt0 n (eq_ind_r (fun n => n > 0) (gt_Sn_O n') E)
+  end eq_refl.
+
+
+Require Import Program.
+
+Program Definition createGt0' (n : nat) : nat :=
+  match n with
+  | O => 42
+  | S n' => useGt0 n _
+  end.
+Next Obligation. apply gt_Sn_O. Qed.
+
+Definition createGt0'' (n : nat) : nat.
+Proof.
+  destruct n eqn:E.
+  - exact 42.
+  - refine (useGt0 n _).
+    rewrite E.
+    apply gt_Sn_O.
+Defined.
